LeanHoG/Invariant/HamiltonianPath/Certificate.lean
@@ -1,29 +1,29 @@
 import Qq
-import LeanHoG.JsonData
 import LeanHoG.Edge
 import LeanHoG.Graph
 import LeanHoG.Util.RB
 import LeanHoG.Util.Quote
-import LeanHoG.Invariant.Hamiltonicity.Basic
+import LeanHoG.Invariant.HamiltonianPath.Basic
+import LeanHoG.Invariant.HamiltonianPath.JsonData
 
 namespace LeanHoG
 
 open Qq
-def hamiltonianPathOfData (G : Q(Graph)) (D : PathData) : Q(HamiltonianPath $G) :=
+def hamiltonianPathOfData (G : Q(Graph)) (D : HamiltonianPathData) : Q(HamiltonianPath $G) :=
   let rec fold (t : Q(Graph.vertex $G)) :
     List Q(Graph.vertex $G) → ((s : Q(Graph.vertex $G)) ×' Q(Walk $G $s $t)) := fun vs =>
     match vs with
     | [] => panic! "Shouldn't be here"
     | [v] =>
       let h : Q($v = $t) := (q(Eq.refl $v) : Lean.Expr)
-      ⟨v, q($h ▸ Walk.trivial $v)⟩
+      ⟨v, q($h ▸ .here $v)⟩
     | u :: v :: vs =>
       let ⟨s, w⟩ := fold t (v :: vs)
       let h : Q(decide (@Graph.adjacent $G $u $s) = true) := (q(Eq.refl true) : Lean.Expr)
-      let w' := q(Walk.left (of_decide_eq_true $h) $w)
+      let w' := q(.step (of_decide_eq_true $h) $w)
       ⟨u, w'⟩
   have n : Q(Nat) := q(Graph.vertexSize $G)
-  let vertices : List Q(Graph.vertex $G) := D.vertices.map (finOfData n)
+  let vertices : List Q(Graph.vertex $G) := D.path.map (finOfData n)
   match vertices.getLast? with
   | none => panic! "no vertices"
   | some t =>
